fairness/comp_utils.v
@@ -1,0 +1,98 @@
+From trillium.fairness Require Import inftraces trace_lookup fairness.
+
+
+Section StepLabelMatches.
+  Context {St L: Type}.
+
+  (* TODO: move *)
+  Definition trace_step: Type := St * option (L * St). 
+
+  Definition step_label_matches (step: trace_step) (P: L -> Prop) :=
+    exists st1 ℓ st2, step = (st1, Some (ℓ, st2)) /\ P ℓ.
+   
+  Instance slm_dec P (DECP: forall ρ, Decision (P ρ)):
+    forall step, Decision (step_label_matches step P).
+  Proof. 
+    rewrite /step_label_matches. intros [? p2].
+    destruct p2 as [p2| ]. 
+    2: { right. intros (?&?&?&?). intuition. congruence. }
+    destruct p2 as [ℓ s2].
+    destruct (decide (P ℓ)).
+    - left. subst. do 2 eexists. eauto.
+    - right. intros (?&?&?&?). intuition. congruence. 
+  Qed. 
+
+  Definition is_end_state (step: trace_step) :=
+    exists st, step = (st, None). 
+
+End StepLabelMatches.
+
+Definition model_trace_step (M: FairModel) := 
+  @trace_step (fmstate M) (option $ fmrole M). 
+
+
+Section ProjectNestedTrace.
+  
+  Context {St L: Type}.
+  Context {St' L': Type}.
+  Context (proj_st: St -> St') (proj_lbl: L -> option L'). 
+  
+  CoFixpoint project_nested_trace (tr: trace St L): trace St' L' :=
+    match tr with 
+    | ⟨ s ⟩ => ⟨ proj_st s ⟩
+    | s -[ ℓ ]-> tr' =>
+        match proj_lbl ℓ with
+        | Some ℓ' => (proj_st s) -[ ℓ' ]-> (project_nested_trace tr')
+        | None => ⟨ proj_st s ⟩
+        end
+    end. 
+
+  Lemma project_nested_trfirst (tr: trace St L):
+    trfirst (project_nested_trace tr) = proj_st (trfirst tr).
+  Proof. 
+    destruct tr; eauto. simpl.
+    by destruct proj_lbl. 
+  Qed. 
+
+  Local Ltac gd t := generalize dependent t.
+
+  Lemma nested_trace_construction (tr: trace St L)
+    (trans: St -> L -> St -> Prop) (trans': St' -> L' -> St' -> Prop)
+    (VALID: trace_valid trans tr)
+    (NESTED_STEPS: ∀ i res, tr !! i = Some res → 
+                         (* is_lib_step res \/ *)
+                         step_label_matches res (is_Some ∘ proj_lbl) \/
+                         is_end_state res)
+    (NESTED_TRANS: forall s1 ℓ s2 ℓ', trans s1 ℓ s2 -> proj_lbl ℓ = Some ℓ' ->
+                                  trans' (proj_st s1) ℓ' (proj_st s2)):
+    (* True.  *)
+    traces_match
+      (* (transA := @ext_trans _ ExtLibLM) *)
+      (* ((option_fmap _ _ inl): option (@ext_role _ ExtLibLM) -> option $ fmrole client_model_impl) *)
+      (* (fun c δ_lib => fst c = δ_lib) *)
+      (* tr *)
+      (* (project_lib_trace tr). *)
+      (fun ℓ ℓ' => proj_lbl ℓ = Some ℓ') (fun st st' => proj_st st = st')
+      trans trans'
+      tr (project_nested_trace tr).
+  Proof.
+    gd tr. cofix IH.
+    intros. 
+    rewrite (trace_unfold_fold (project_nested_trace tr)).
+    destruct tr.
+    { econstructor. done. }
+    (* do 2 red. *)
+    pose proof (NESTED_STEPS 0 (s, Some (ℓ, (trfirst tr))) eq_refl) as STEP0.
+    destruct STEP0 as [STEP0 | STEP0].
+    2: { destruct STEP0. done. }
+    destruct STEP0 as (?&?&?&[=]&[ℓ' PROJ]). subst. simpl in *.
+    pose proof (trace_valid_cons_inv _ _ _ _ VALID) as [VALID' STEP].
+    rewrite PROJ. econstructor.
+    1-3: done.
+    { rewrite project_nested_trfirst. eauto. }
+    eapply IH; eauto. intros. 
+    apply (NESTED_STEPS (S i)); eauto. 
+  Qed.
+
+End ProjectNestedTrace.
+
